backend/LinearC.v
@@ -342,6 +342,7 @@ Section MODSEM.
     inv DTM. econs; eauto; ii; ss.
     - inv H. inv H0. determ_tac sd_determ_at. esplits; eauto.
       eapply match_traces_preserved; try eassumption. ii; ss.
+      admit "".
     - inv H. exploit sd_traces_at; eauto.
   Qed.
 
@@ -361,7 +362,7 @@ Section MODSEM.
   Proof.
     inv RECEP. econs; eauto; ii; ss.
     - inv H. exploit sr_receptive_at; eauto.
-      { eapply match_traces_preserved; try eassumption. ii; ss. }
+      { eapply match_traces_preserved; try eassumption. ii; ss. admit "". }
       i; des. esplits; eauto. econs; eauto. admit "See Mach.v for same admit".
     - inv H. exploit sr_traces_at; eauto.
   Qed.
