common/EventsC.v
@@ -1,0 +1,40 @@
+Require Import String.
+Require Import CoqlibC.
+Require Intv.
+Require Import AST.
+Require Import Integers.
+Require Import Floats.
+Require Import Values.
+Require Import Memory.
+Require Import Globalenvs.
+(** newly added **)
+Require Export Events.
+
+Set Implicit Arguments.
+
+
+
+Lemma eventval_valid_le
+      se_small ev se_big
+      (VALID: eventval_valid se_small ev)
+      (LE: se_small.(Senv.public_symbol) <1= se_big.(Senv.public_symbol))
+  :
+    <<VALID: eventval_valid se_big ev>>
+.
+Proof.
+  u in *.
+  unfold eventval_valid in *. des_ifs. erewrite LE; eauto.
+Qed.
+
+Lemma match_traces_le
+      se_small tr0 tr1 se_big
+      (MATCH: match_traces se_small tr0 tr1)
+      (LE: se_small.(Senv.public_symbol) <1= se_big.(Senv.public_symbol))
+  :
+    <<MATCH: match_traces se_big tr0 tr1>>
+.
+Proof.
+  u in *.
+  inv MATCH; econs; eauto; eapply eventval_valid_le; eauto.
+Qed.
+
