proof/SemProps.v
@@ -6,7 +6,7 @@ Require Import Values.
 Require Import JMeq.
 Require Import Smallstep.
 Require Import Integers.
-Require Import Events.
+Require Import EventsC.
 Require Import MapsC.
 
 Require Import Skeleton ModSem Mod Sem.
@@ -299,31 +299,6 @@ End INITDTM.
 
 
 
-
-(* TODO: Move to EventsC *)
-Lemma eventval_valid_le
-      se_small ev se_big
-      (VALID: eventval_valid se_small ev)
-      (LE: se_small.(Senv.public_symbol) <1= se_big.(Senv.public_symbol))
-  :
-    <<VALID: eventval_valid se_big ev>>
-.
-Proof.
-  u in *.
-  unfold eventval_valid in *. des_ifs. erewrite LE; eauto.
-Qed.
-
-Lemma match_traces_le
-      se_small tr0 tr1 se_big
-      (MATCH: match_traces se_small tr0 tr1)
-      (LE: se_small.(Senv.public_symbol) <1= se_big.(Senv.public_symbol))
-  :
-    <<MATCH: match_traces se_big tr0 tr1>>
-.
-Proof.
-  u in *.
-  inv MATCH; econs; eauto; eapply eventval_valid_le; eauto.
-Qed.
 
 Lemma lift_step
       (ms: ModSem.t) st0 tr st1
